Finish a proof in Trace.v

src/Spec/Trace.v
@@ -1,5 +1,7 @@
 Require Import Coq.Lists.List.
 Require Import Crypto.Util.Decidable.
+Require Import Crypto.Util.Tactics.DestructHead.
+Require Import Crypto.Util.Tactics.SpecializeBy.
 
 Section Trace.
   Context {state input output : Type}
@@ -11,9 +13,9 @@ Section Trace.
                    (_:multistep s0 l s1)
                    (_:step s1 i o s2) :
       multistep s0 (l++(i,o)::nil) s2.
-  (* FIXME: maybe replace with invariant definition *)
+
   Definition allows_behavior l :=
-    exists s0 s1, init s0 -> multistep s0 l s1.
+    exists s0 s1, init s0 /\ multistep s0 l s1.
 End Trace.
 
 (* 1. Synthesize "intersection negotiation" of options, e.g., choose
@@ -34,19 +36,77 @@ Definition output_in_list_and_previous_input_matching_satisfies
     List.In message trace
     -> matcher (snd message)
     -> exists other_message : input * output,
-        R (fst other_message) (snd message).
+        List.In other_message trace
+        /\ R (fst other_message) (snd message).
+
+Lemma output_in_list_and_previous_input_matching_satisfies_nil
+      {input output matcher R}
+  : @output_in_list_and_previous_input_matching_satisfies input output matcher R nil.
+Proof.
+  intros ? H; inversion H.
+Qed.
+
+Lemma output_in_list_and_previous_input_matching_satisfies_snoc
+      {input output matcher R}
+      trace msg
+  : @output_in_list_and_previous_input_matching_satisfies input output matcher R trace
+    -> (matcher (snd msg)
+        -> exists other_message,
+           List.In other_message (trace ++ (msg::nil))
+           /\ R (fst other_message) (snd msg))
+    -> @output_in_list_and_previous_input_matching_satisfies input output matcher R (trace ++ (msg::nil)).
+Proof.
+  unfold output_in_list_and_previous_input_matching_satisfies.
+  setoid_rewrite in_app_iff; simpl.
+  intros H0 H1 message Hin Hmatcher.
+  destruct_head'_or; destruct_head' False; subst; eauto.
+  { specialize (H0 message); specialize_by_assumption.
+    destruct_head'_ex; destruct_head'_and; eauto. }
+Qed.
 
 Section Example_1_Negotiation.
   Definition trace_satisfies_negotiation_spec
              (trace : list (list nat (*input*) * nat (*output*))) : Prop
     := output_in_list_and_previous_input_matching_satisfies
          (fun output => True)
-         (fun i o => List.In o i)
+         (fun i o => i <> nil -> List.In o i)
          trace.
 End Example_1_Negotiation.
 
 Section Example_1_Negotiation_Synthesis.
   Opaque output_in_list_and_previous_input_matching_satisfies.
+
+  Lemma handle_stateless {state input output init}
+        {trace matcher} {R : _ -> _ -> Prop}
+        (handler : input -> output)
+        (step : state -> input -> output -> state -> Prop
+         := fun _ i o _ => handler i = o)
+        (handler_ok : forall i, R i (handler i))
+    : (forall st0 st1 io, step st0 (fst io) (snd io) st1
+                          -> R (fst io) (snd io))
+      -> (@allows_behavior state input output init step trace
+          -> output_in_list_and_previous_input_matching_satisfies
+               matcher R trace).
+  Proof.
+    subst step; cbv beta.
+    intros Hstep Hbehavior.
+    repeat first [ progress destruct_head_hnf' ex
+                 | progress destruct_head'_and ].
+    let H := match goal with H : multistep _ _ _ _ |- _ => H end in
+    induction H as [|??????? IH]; subst.
+    { apply output_in_list_and_previous_input_matching_satisfies_nil. }
+    { repeat first [ progress specialize_by_assumption
+                   | assumption
+                   | apply output_in_list_and_previous_input_matching_satisfies_snoc
+                   | setoid_rewrite List.in_app_iff
+                   | intro
+                   | eexists
+                   | apply conj
+                   | eapply (Hstep (_, _)); simpl; reflexivity
+                   | solve [ auto ]
+                   | progress simpl ]. }
+  Qed.
+
   Goal { state : Type
      & { init : state -> Prop
      & { step : _
@@ -67,23 +127,14 @@ Section Example_1_Negotiation_Synthesis.
       end.
     start.
     start_unfold.
-    Lemma handle_stateless {state input output init}
-          {trace matcher} {R : _ -> _ -> Prop}
-          (handler : input -> output)
-          (step : state -> input -> output -> state -> Prop
-           := fun _ i o _ => handler i = o)
-          (handler_ok : forall i, R i (handler i))
-      : (forall st0 st1 io, step st0 (fst io) (snd io) st1
-                            -> R (fst io) (snd io))
-        -> (@allows_behavior state input output init step trace
-            -> output_in_list_and_previous_input_matching_satisfies
-                 matcher R trace).
-    Proof.
-      subst step; cbv beta.
-      intros Hstep Hbehavior.
-      Require Import Crypto.Util.Tactics.DestructHead.
-      destruct_head_hnf' ex.
-
-    Abort.
-  Abort.
+    { eapply handle_stateless.
+      Lemma handle_membership_with_first {T} (default : T)
+        : forall i : list T, i <> nil -> In (hd default i) i.
+      Proof. intros [|? ?] ?; simpl; auto; congruence. Qed.
+      apply (handle_membership_with_first 0).
+      intros ?? [ls ?] ?; simpl in *; subst; apply handle_membership_with_first. }
+    Grab Existential Variables.
+    exact (fun _ => True).
+    exact unit.
+  Defined.
 End Example_1_Negotiation_Synthesis.
